examples/mutsum/MutMainA.v
@@ -21,9 +21,6 @@ Module MutMainA. Section MutMainA.
   Definition Spc: alist string fspec :=
     Seal.sealing CRIS [(MutMainName.main, main_spec)].
 
-  Lemma Spc_nodup: List.NoDup (List.map fst Spc).
-  Proof. unfold Spc. unseal CRIS. prove_nodup. Qed.
-
   Definition fnsems :=
     [(MutMainName.main, (scopes, mk_specbody main_spec main_body))].
 
@@ -36,7 +33,7 @@ Module MutMainA. Section MutMainA.
   Solve All Obligations with prove_scope.
   Next Obligation. prove_nodup. Qed.
 
-  Definition InitCond : iProp := emp%I.
+  Definition init_cond : iProp := emp%I.
 
   Definition t u Spc := Seal.sealing CRIS (SMod.to_hmod (wsim_ginv u ⊤) Spc Mod).
 End MutMainA. End MutMainA.
