examples/cannon/CannonMainIAproof.v
@@ -24,12 +24,22 @@ Module CannonMainIA. Section CannonMainIA.
   Lemma simF_main : HSim.sim_fun open MainAMod MainIMod Ist MainName.main.
   Proof.
     winit_simF 0 0.
+
+    (* SRC: precondition *)
     wsteps_l. iDestruct "ASM" as "((%Y & B) & %Q)". subst. hss.
-    wsteps_r. 
-    unfold HoareCall. wforce_l. instantiate (1:=()). wforce_l.
+
+    (* SRC: prove the precondition of "fire" *)
+    wsteps_r. unfold HoareCall. wforce_l. instantiate (1:=()). wforce_l.
     wforce_l. iSplitL "B"; et. wsteps_l.
+
+    (* SRC, TGT; call "fire" and take a postcondition *)
     wcall "IST"; et. wsteps_l. iDestruct "ASM" as "[% %]"; des; subst. hss.
-    wsteps_r. hss. wsteps_r. wstep. wsteps_l. wsteps_r. wforce_l.
+    wsteps_r. hss. wsteps_r.
+    
+    (* SRC, TGT: print 1 *)
+    wstep. wsteps_l. wsteps_r. wforce_l.
+
+    (* SRC: prove the postcondition & IST *)
     wforce_l. iSplitR; et. wsteps_l.
     wstep. iFrame; et.
   Qed.
