examples/spinlock/SpinLockIAProof.v
@@ -49,7 +49,7 @@ Module SpinLockIA. Section SpinLockIA.
     wforces_l. iFrame. iSplit; eauto.
     { iSplit; eauto. rewrite /is_lock. iExists _, _; iSplit; eauto. }
     wsteps_l. wstep. eauto.
-  (*FAST*)Admitted.
+  (*FAST*)Qed.
 
   Lemma acquire_simF : HSim.sim_fun open MA MI IstFull SpinLockName.acquire.
   Proof.
@@ -108,7 +108,7 @@ Module SpinLockIA. Section SpinLockIA.
       (* both terminate *)
       wstep; eauto.
     }
-  (*FAST*)Admitted.
+  (*FAST*)Qed.
 
   Lemma release_simF : HSim.sim_fun open MA MI IstFull SpinLockName.release.
     winit_simF u_a 0.
@@ -139,7 +139,7 @@ Module SpinLockIA. Section SpinLockIA.
       iDestruct "UNLOCKED" as "[POINTS_TO [Q' TKN']]".
       iCombine "TKN TKN'" gives %Hv. done.
     }
-  (*FAST*)Admitted.
+  (*FAST*)Qed.
 
   (* Construct HSim.t for summing up each simulation proofs *)
   Lemma sim : HSim.t open MA MI emp%I IstFull.
